theorems/iN/iN_lemmas.lean
@@ -1,17 +1,22 @@
 import theorems.iN.SimpSets
 import theorems.iN.iN_def
-import theorems.iN.iN_tactics
 import theorems.iN.iN_rewrite
 import theorems.Core.Attrs.Attrs
 
 /-- The supported bit sizes. Proofs do not need to prove ∀n : Nat. -/
 inductive Bits : Nat → Prop where
-  | i1 : Bits 1
   | i8 : Bits 8
   | i16 : Bits 16
   | i32 : Bits 32
   | i64 : Bits 64
-  | i128 : Bits 128
+
+/-- The supported bit sizes, with bool. Proofs do not need to prove ∀n : Nat. -/
+inductive BitsBool : Nat → Prop where
+  | i1 : BitsBool 1
+  | i8 : BitsBool 8
+  | i16 : BitsBool 16
+  | i32 : BitsBool 32
+  | i64 : BitsBool 64
 
 @[grind =]
 theorem BitVec.saddOverflow_comm {n} (a b : BitVec n)
@@ -29,7 +34,7 @@ theorem BitVec.uaddOverflow_comm {n} (a b : BitVec n)
   unfold BitVec.uaddOverflow
   grind
 
-theorem BitVec.saddOverflow_chain_assoc_monotone {n} {hn : Bits n} (a b c : BitVec n)
+theorem BitVec.saddOverflow_chain_assoc_monotone {n} {hn : BitsBool n} (a b c : BitVec n)
     (h : a.msb = b.msb ∧ b.msb = c.msb)
 
     : (a.saddOverflow b || (a + b).saddOverflow c) =
@@ -41,7 +46,7 @@ theorem BitVec.saddOverflow_chain_assoc_monotone {n} {hn : Bits n} (a b c : BitV
   case i16  => bv_check "../../lrat/BitVec.saddOverflow_assoc_monotone-47-15.lrat"
   case i32  => bv_check "../../lrat/BitVec.saddOverflow_assoc_monotone-48-15.lrat"
   case i64  => bv_check "../../lrat/BitVec.saddOverflow_assoc_monotone-49-15.lrat"
-  case i128 => bv_check "../../lrat/BitVec.saddOverflow_assoc_monotone-50-15.lrat"
+  --case i128 => bv_check "../../lrat/BitVec.saddOverflow_assoc_monotone-50-15.lrat"
 
 /- theorem test : ∃ (n : Nat) (a b c : BitVec n),
     ¬((a.saddOverflow b || (a + b).saddOverflow c) ==
@@ -49,7 +54,7 @@ theorem BitVec.saddOverflow_chain_assoc_monotone {n} {hn : Bits n} (a b c : BitV
 
   exists 8, 127#8, 1#8, -1#8 -/
 
-theorem BitVec.uaddOverflow_chain_assoc {n} {hn : Bits n} (a b c : BitVec n)
+theorem BitVec.uaddOverflow_chain_assoc {n} {hn : BitsBool n} (a b c : BitVec n)
     : (a.uaddOverflow b || (a + b).uaddOverflow c) =
       (b.uaddOverflow c || a.uaddOverflow (b + c)) := by
 
@@ -59,202 +64,25 @@ theorem BitVec.uaddOverflow_chain_assoc {n} {hn : Bits n} (a b c : BitVec n)
   case i16  => bv_check "../../lrat/iN_lemmas.lean-BitVec.uaddOverflow_chain_assoc-59-15.lrat"
   case i32  => bv_check "../../lrat/iN_lemmas.lean-BitVec.uaddOverflow_chain_assoc-60-15.lrat"
   case i64  => bv_check "../../lrat/iN_lemmas.lean-BitVec.uaddOverflow_chain_assoc-61-15.lrat"
-  case i128 => bv_check "../../lrat/iN_lemmas.lean-BitVec.uaddOverflow_chain_assoc-62-16.lrat"
+  --case i128 => bv_check "../../lrat/iN_lemmas.lean-BitVec.uaddOverflow_chain_assoc-62-16.lrat"
 
-namespace iN
+/- theorem BitVec.saddOverflow_chain_assoc_monotone {n} {hn : Bits n} (a b c : BitVec n)
+    (h : a.msb = b.msb ∧ b.msb = c.msb)
 
-@[simp, grind =]
-theorem eq_bitvec_inj {n} {a b : BitVec n} :
-    ((bitvec a : iN n) = (bitvec b : iN n)) ↔ a = b := by
-
-  constructor
-  · intro h
-    injection h
-  . intro h
-    rw [h]
-
-@[simp]
-theorem poisonWrapper_poison_left {n} {k} {g : BitVec n → BitVec n → iN k} {b : iN n} :
-  iN.poisonWrapper g poison b = poison := by simp [iN.poisonWrapper]
-
-@[simp]
-theorem poisonWrapper_poison_right {n} {k} {g : BitVec n → BitVec n → iN k} {a : iN n} :
-  iN.poisonWrapper g a poison = poison := by cases a <;> rfl
-
-@[simp]
-theorem poisonWrapper_bitvec_left {n} {k} {g : BitVec n → BitVec n → iN k} {a : BitVec n} {b : iN n} :
-  iN.poisonWrapper g (bitvec a) b = match b with
-    | poison => poison
-    | bitvec b' => g a b' := by cases b <;> rfl
-
-@[simp]
-theorem poisonWrapper_bitvec_right {n} {k} {g : BitVec n → BitVec n → iN k} {a : iN n} {b : BitVec n} :
-  iN.poisonWrapper g a (bitvec b) = match a with
-    | poison => poison
-    | bitvec a' => g a' b := by cases a <;> rfl
-
-@[simp]
-theorem poisonWrapper_bitvec {n} {k} {g : BitVec n → BitVec n → iN k} {a b : BitVec n} :
-  iN.poisonWrapper g (bitvec a) (bitvec b) = g a b := by cases a <;> rfl
-
-/-- Simplifying lemma about poisonable equations of the form `(a ⋄₁ b) ⋄₂ c`. -/
-@[simp]
-theorem poisonPreconditions_match_wrapper_assoc_left {n}
-    (isPoison₁ : BitVec n → BitVec n → Bool)
-    (isPoison₂ : BitVec n → BitVec n → Bool)
-    (a b c : BitVec n)
-    (op₁ : BitVec n → BitVec n → BitVec n)
-    (op₂ : BitVec n → BitVec n → BitVec n)
-    : (match iN.poisonPreconditions isPoison₁ op₁ a b with
-      | poison => poison
-      | bitvec ab' => iN.poisonPreconditions isPoison₂ op₂ ab' c)
-
-      = bif isPoison₁ a b || isPoison₂ (op₁ a b) c then
-        poison
-      else
-        bitvec (op₂ (op₁ a b) c) := by
-
-  unfold iN.poisonPreconditions
-  cases isPoison₁ a b
-  . simp
-  . simp
-
-/-- Simplifying lemma about poisonable equations of the form `a ⋄₁ (b ⋄₂ c)`. -/
-@[simp]
-theorem poisonPreconditions_match_wrapper_assoc_right {n}
-    (isPoison₁ : BitVec n → BitVec n → Bool)
-    (isPoison₂ : BitVec n → BitVec n → Bool)
-    (a b c : BitVec n)
-    (op₁ : BitVec n → BitVec n → BitVec n)
-    (op₂ : BitVec n → BitVec n → BitVec n)
-    : (match iN.poisonPreconditions isPoison₂ op₂ b c with
-      | poison => poison
-      | bitvec bc' => iN.poisonPreconditions isPoison₁ op₁ a bc')
-
-      = bif isPoison₂ b c || isPoison₁ a (op₂ b c) then
-        poison
-      else
-        bitvec (op₁ a (op₂ b c)) := by
-
-  unfold iN.poisonPreconditions
-  cases isPoison₂ b c
-  . simp
-  . simp
-
-@[simp]
-theorem bitvec_cond {n} (c : Bool) (t e : BitVec n) :
-    cond c (bitvec t) (bitvec e) = bitvec (cond c t e) := by
-  cases c <;> rfl
-
-/-- Forces unfolds when about to be simplified -/
-@[simp]
-theorem poisonPreconditions_rewrite_unfold {n} (a b : BitVec n) (c : iN n)
-    (isPoison : BitVec n → BitVec n → Bool) (op : BitVec n → BitVec n → BitVec n)
-    : (iN.poisonPreconditions isPoison op a b ~> c) =
-      ((if isPoison a b then poison else bitvec (op a b)) ~> c) := by
-
-  unfold iN.poisonPreconditions
-  rfl
-
-/-- Forces unfolds when about to be simplified -/
-@[simp]
-theorem poisonPreconditions_rewrite_iff_unfold_left {n} (a b : BitVec n) (c : iN n)
-    (isPoison : BitVec n → BitVec n → Bool) (op : BitVec n → BitVec n → BitVec n)
-    : (iN.poisonPreconditions isPoison op a b <~> c) =
-      ((if isPoison a b then poison else bitvec (op a b)) <~> c) := by
-
-  unfold iN.poisonPreconditions
-  rfl
-
-/-- Forces unfolds when about to be simplified -/
-@[simp]
-theorem poisonPreconditions_rewrite_iff_unfold_right {n} (a b : BitVec n) (c : iN n)
-    (isPoison : BitVec n → BitVec n → Bool) (op : BitVec n → BitVec n → BitVec n)
-    : (c <~> iN.poisonPreconditions isPoison op a b) =
-      (c <~> (if isPoison a b then poison else bitvec (op a b))) := by
-
-  unfold iN.poisonPreconditions
-  rfl
-
-/- @[grind =]
-theorem addNswBV_comm {n} {a b : BitVec n}
-    : iN.addNswBV a b = iN.addNswBV b a := by
-
-  simp only [iN_to_bitvec]
-  rw [BitVec.saddOverflow_comm]
-  split <;> try simp
-
-  -- h✝ : ¬b.saddOverflow a = true
-  -- ⊢ a + b = b + a
-  grind
-
-@[grind =]
-theorem addNuwBV_comm {n} {a b : BitVec n}
-    : iN.addNuwBV a b = iN.addNuwBV b a := by
-
-  simp only [iN_to_bitvec]
-  rw [BitVec.uaddOverflow_comm]
-  split <;> try simp
-
-  -- h✝ : ¬b.uaddOverflow a = true
-  -- ⊢ a + b = b + a
-  grind -/
-
-end iN
-
-/- @[grind =]
-theorem saddOverflow_comm_tete {n} (a b : BitVec n)
-    : a.saddOverflow b = true ↔ b.saddOverflow a = true := by
-
-  unfold BitVec.saddOverflow at *
-  grind -/
-
-/- theorem saddOverflow_contra {n} (a b : BitVec n)
-    :  -/
-
-/- @[simp]
-theorem iN_contra {n} {a : BitVec n}
-    {h : (poison : iN n) = (bitvec a : iN n)} : False := by
-
-  cases h -/
-
-/- theorem test_without {n} (x : iN n) : iN.shlNsw x 0 = x := by
-  simp [iN_unwrap_poison]
-  cases x with
-  | poison => rfl
-  | bitvec a => simp [iN_to_bitvec]
-
-/- theorem com {n} (x y : iN n)
-    : x + y = y + x := by
-
-  cases x with
-  | poison => rfl
-
-  simp [iN_to_bitvec]
+    : (a.saddOverflow b || (a + b).saddOverflow c) =
+      (b.saddOverflow c || a.saddOverflow (b + c)) := by
  -/
 
-/- @[simp]
-theorem com {n} (x : iN n) (val : Nat)
-  : ((no_index OfNat.ofNat val) : iN n) + x
-    = x + ((no_index OfNat.ofNat val) : iN n) := by
-  cases x with
-  | poison => rfl
-  | bitvec a =>
-    simp [iN_to_bitvec]
-    apply BitVec.add_comm -/
+@[simp]
+theorem sadd_overflow_assoc_of_nonneg (a b c : BitVec 32) :
+  a.slt 0#32 = false → b.slt 0#32 = false → c.slt 0#32 = false →
+  ((a.saddOverflow b || (a + b).saddOverflow c) ↔ (b.saddOverflow c || a.saddOverflow (b + c))) := by
 
+  bv_decide
 
 @[simp]
-theorem com0 {n} (x : iN n) (val : Nat)
-  : lit(val) + x = x + lit(val) := by
-  cases x with
-  | poison => rfl
-  | bitvec a =>
-    simp [iN_to_bitvec]
-    apply BitVec.add_comm
+theorem sadd_overflow_assoc_of_neg (x y z : BitVec 32) :
+  x.slt 0#32 = true → y.slt 0#32 = true → z.slt 0#32 = true →
+  ((x.saddOverflow y || (x + y).saddOverflow z) ↔ (y.saddOverflow z || x.saddOverflow (y + z))) := by
 
--- @bitvec n 23#↑n : iN n
-
-theorem test {n} (x : iN n) : x + x = x + 23 := by
-
-  simp -/
+  bv_decide
