theorems/iN/SimpSets.lean
@@ -2,6 +2,10 @@ import Lean
 
 open Lean Meta
 
-initialize iNInst : SimpExtension ←
+/- initialize iNInst : SimpExtension ←
   registerSimpAttr `iN_unwrap_inst
+    "simp lemmas unwrapping instructions" -/
+
+initialize iNInst : SimpExtension ←
+  registerSimpAttr `simp_iN
     "simp lemmas unwrapping instructions"
