theorems/iN/iN_rewrite.lean
@@ -10,24 +10,18 @@ inductive Rewrite {n} : iN n → iN n → Prop where
   | poison_forge (v : BitVec n) : Rewrite poison (bitvec v)
 
 /--
-`RewriteReverse x y` means the value `y` can be rewritten into the value `x`.
--/
-abbrev RewriteReverse {n} (x y : iN n) := Rewrite y x
-
-/--
 `RewriteIff x y` means `x` can be rewritten into `y` and `y` can be rewritten into `x`.
 -/
 abbrev RewriteIff {n} (x y : iN n) := Rewrite x y ∧ Rewrite y x
 
 @[inherit_doc] infix:50 " ~> "  => Rewrite
-@[inherit_doc] infix:50 " <~ "  => RewriteReverse
 @[inherit_doc] infix:50 " <~> " => RewriteIff
 
 namespace Rewrite
 
 /-- Poison can be rewritten to anything. -/
-@[simp, grind]
-theorem rewrite_poison {n} (x : iN n)
+@[simp]
+theorem poison_rewrite {n} (x : iN n)
     : poison ~> x := by
 
   cases x
@@ -36,16 +30,30 @@ theorem rewrite_poison {n} (x : iN n)
   case poison =>
     exact Rewrite.refl poison
 
-/-- Poison can be rewritten to anything. -/
-@[simp, grind]
+/-- Values cannot be rewritten to poison. -/
+@[simp]
 theorem not_bitvec_poision_rewrite {n} (a : BitVec n)
     : ¬bitvec a ~> poison := by
 
   intro h
   cases h
 
+@[simp]
+theorem rewrite_poison_iff {n} {x : iN n}
+    : (x ~> poison) ↔ (x = poison) := by
+
+  constructor
+  case mp =>
+    intro h
+    cases h
+    case refl => rfl
+  case mpr =>
+    intro h
+    rw [h]
+    exact Rewrite.refl poison
+
 @[refl, simp]
-theorem rewrite_refl {n} {x : iN n}
+theorem rewrite_refl {n} (x : iN n)
     : x <~> x := by
 
   constructor <;> exact Rewrite.refl x
@@ -55,8 +63,13 @@ theorem rewrite_refl2 {n} {x : iN n}
     : Rewrite x x ∧ Rewrite x x := by
 
   -- this handles cases after the `abbrev` is unwrapped
-
   constructor <;> exact Rewrite.refl x
+
+instance {n} : @Std.Refl (iN n) Rewrite where
+  refl := Rewrite.refl
+
+instance {n} : @Std.Refl (iN n) RewriteIff where
+  refl x := Rewrite.rewrite_refl x
 
 @[grind →]
 theorem rewrite_trans {n} {x y z : iN n}
@@ -66,7 +79,7 @@ theorem rewrite_trans {n} {x y z : iN n}
   case refl =>
     exact hy
   case poison_forge v =>
-    exact rewrite_poison z
+    exact poison_rewrite z
 
 @[grind]
 theorem eq_rewrite {n} {x y : iN n}
@@ -92,7 +105,7 @@ theorem eq_iff_rewrite_bitvec {n} {a b : BitVec n}
       rfl
 
 @[simp, grind]
-theorem rewrite_bitvec {n} (a b : BitVec n)
+theorem rewrite_bitvec_bitvec {n} (a b : BitVec n)
     : (bitvec a ~> bitvec b) ↔ a = b := by
 
   constructor
@@ -104,5 +117,170 @@ theorem rewrite_bitvec {n} (a b : BitVec n)
     intro h
     rw [h]
     exact Rewrite.refl (bitvec b)
+
+@[simp, grind]
+theorem rewrite_bitvec_iN {n} (a : BitVec n) (y : iN n)
+    : (bitvec a ~> y) ↔ y = bitvec a := by
+
+  constructor
+  case mp =>
+    intro h
+    cases h
+    case refl => rfl
+  case mpr =>
+    intro h
+    rw [h]
+    exact Rewrite.refl (bitvec a)
+
+@[simp]
+theorem if_then_poison_rewrite_iff {n} (c : Prop) [Decidable c] (x y : iN n)
+    : (if c then poison else x : no_index _) ~> y ↔ ¬c → x ~> y := by
+
+  split <;> simp [*]
+
+@[simp]
+theorem bitvec_rewrite_if_then_poison_iff {n} (a : BitVec n) (c : Prop) [Decidable c] (y : iN n)
+    : bitvec a ~> (if c then poison else y : no_index _) ↔ ¬c ∧ bitvec a ~> y := by
+
+  split <;> simp [*]
+
+@[simp]
+theorem if_then_rewrite_if_then_iff {n} (c : Prop) [Decidable c] (x1 x2 y1 y2 : iN n)
+    : (if c then x1 else x2 : no_index _) ~> (if c then y1 else y2 : no_index _) ↔
+      (c → x1 ~> y1) ∧ (¬c → x2 ~> y2) := by
+
+  split <;> simp [*]
+
+@[simp]
+theorem if_then_rewrite_iff {n} (c : Prop) [Decidable c] (x1 x2 y : iN n)
+    : (if c then x1 else x2 : no_index _) ~> y ↔
+      (c → x1 ~> y) ∧ (¬c → x2 ~> y) := by
+
+  split <;> simp [*]
+
+@[simp]
+theorem rewrite_if_then_iff {n} (c : Prop) [Decidable c] (x : iN n) (y1 y2 : iN n)
+    : x ~> (if c then y1 else y2 : no_index _) ↔
+      (c → x ~> y1) ∧ (¬c → x ~> y2) := by
+
+  split <;> simp [*]
+
+-- recreate the above for RewriteIff
+@[simp, grind]
+theorem rewrite_iff_bitvec_bitvec {n} (a b : BitVec n)
+    : (bitvec a <~> bitvec b) ↔ a = b := by
+
+  constructor
+  case mp =>
+    intro h
+    cases h with
+    | intro hab hba =>
+      cases hab
+      cases hba
+      rfl
+  case mpr =>
+    intro h
+    rw [h]
+
+@[simp, grind]
+theorem rewrite_iff_bitvec_iN {n} (a : BitVec n) (y : iN n)
+    : (bitvec a <~> y) ↔ y = bitvec a := by
+
+  constructor
+  case mp =>
+    intro h
+    cases h with
+    | intro hab hba =>
+      cases hab
+      cases hba
+      rfl
+  case mpr =>
+    intro h
+    rw [h]
+
+@[simp]
+theorem bitvec_rewrite_iff_if_then_poison_iff {n} (a : BitVec n) (c : Prop) [Decidable c] (y : iN n)
+    : bitvec a <~> (if c then poison else y : no_index _) ↔ ¬c ∧ bitvec a ~> y := by
+
+  split <;> simp [*]
+
+@[simp]
+theorem if_then_rewrite_iff_if_then_iff {n} (c : Prop) [Decidable c] (x1 x2 y1 y2 : iN n)
+    : (if c then x1 else x2 : no_index _) <~> (if c then y1 else y2 : no_index _) ↔
+      (c → x1 <~> y1) ∧ (¬c → x2 <~> y2) := by
+
+  split <;> simp [*]
+
+@[simp]
+theorem if_then_rewrite_iff_iff {n} (c : Prop) [Decidable c] (x1 x2 y : iN n)
+    : (if c then x1 else x2 : no_index _) <~> y ↔
+      (c → x1 <~> y) ∧ (¬c → x2 <~> y) := by
+
+  split <;> simp [*]
+
+@[simp]
+theorem rewrite_iff_if_then_iff {n} (c : Prop) [Decidable c] (x : iN n) (y1 y2 : iN n)
+    : x <~> (if c then y1 else y2 : no_index _) ↔
+      (c → x <~> y1) ∧ (¬c → x <~> y2) := by
+
+  split <;> simp [*]
+
+@[simp]
+theorem poison_rewrite_iff {n} {x : iN n}
+    : (poison <~> x) ↔ (x = poison) := by
+
+  constructor
+  case mp =>
+    intro h
+    cases h
+    simp_all
+  case mpr =>
+    intro h
+    rw [h]
+
+@[simp]
+theorem rewrite_iff_poison {n} (x : iN n)
+    : (x <~> poison) ↔ (x = poison) := by
+
+  constructor
+  case mp =>
+    intro h
+    cases h
+    simp_all
+  case mpr =>
+    intro h
+    rw [h]
+
+@[simp]
+theorem bitvec_rewrite_poison_iff {n} (a : BitVec n)
+    : (bitvec a <~> poison) ↔ False := by
+
+  constructor
+  case mp =>
+    intro h
+    cases h
+    simp_all
+  case mpr =>
+    intro h
+    cases h
+
+@[simp]
+theorem poison_rewrite_bitvec_iff {n} (a : BitVec n)
+    : (poison <~> bitvec a) ↔ False := by
+
+  constructor
+  case mp =>
+    intro h
+    cases h
+    simp_all
+  case mpr =>
+    intro h
+    cases h
+
+@[simp]
+theorem poison_rewrite_poison_iff {n}
+    : ((poison : iN n) <~> poison) := by
+
+  constructor <;> exact Rewrite.refl poison
 
 end Rewrite
