theorems/iN_basic/add.lean
@@ -2,124 +2,40 @@ import theorems.iN.iN
 
 namespace iN
 
--- TODO mark not `@[rewrite]` but something for directional equality
+theorem add_comm {hn : Bits n} (x y : iN n)
+    : x + y <~> y + x := by blast hn
+
+theorem addNsw_comm {hn : Bits n} (x y : iN n)
+    : x +nsw y <~> y +nsw x := by blast hn
+
+theorem addNuw_comm {hn : Bits n} (x y : iN n)
+    : x +nuw y <~> y +nuw x := by blast hn
+
+theorem addNw_comm {hn : Bits n} (x y : iN n)
+    : x +nw y <~> y +nw x := by blast hn
+
+theorem addNsw_refine (x y : iN n)
+  : x +nsw y ~> x + y := by blast hn
+
+theorem addNuw_refine (x y : iN n)
+  : x +nuw y ~> x + y := by blast hn
+
+theorem addNw_refine (x y : iN n)
+  : x +nw y ~> x + y := by blast hn
+
+theorem add_assoc {hn : Bits n} (x y z : iN n)
+    : (x + y) + z <~> x + (y + z) := by blast hn
 
 @[grind]
-theorem add_comm {n} (x y : iN n)
-    : x + y = y + x := by
-
-  poison_unroll x y => a b
-  simp [iN_unwrap_inst]
-  rw [BitVec.add_comm a b]
-
-@[grind]
-theorem addNsw_comm {n} (x y : iN n)
-    : x +nsw y <~> y +nsw x := by
-
-  poison_unroll x y => a b
-  simp [iN_unwrap_inst]
-  rw [BitVec.saddOverflow_comm a b]
-  rw [BitVec.add_comm a b]
-
-@[grind]
-theorem addNuw_comm {n} (x y : iN n)
-    : x +nuw y <~> y +nuw x := by
-
-  poison_unroll x y => a b
-  simp [iN_unwrap_inst]
-  rw [BitVec.uaddOverflow_comm a b]
-  rw [BitVec.add_comm a b]
-
-@[grind]
-theorem addNw_comm {n} (x y : iN n)
-    : x +nw y <~> y +nw x := by
-
-  poison_unroll x y => a b
-  simp [iN_unwrap_inst]
-  rw [BitVec.add_comm a b]
-  rw [BitVec.saddOverflow_comm a b]
-  rw [BitVec.uaddOverflow_comm a b]
-
-@[grind]
-theorem addNsw_refine {n} (x y : iN n)
-  : x +nsw y ~> x + y := by
-
-  poison_unroll x y => a b
-
-  simp [iN_unwrap_inst]
-  if h : a.saddOverflow b then
-    simp [h]
-  else
-    simp [h]
-
-@[grind]
-theorem addNuw_refine {n} (x y : iN n)
-  : x +nuw y ~> x + y := by
-
-  poison_unroll x y => a b
-
-  simp [iN_unwrap_inst]
-  if h : a.uaddOverflow b then
-    simp [h]
-  else
-    simp [h]
-
-@[grind]
-theorem addNw_refine {n} (x y : iN n)
-  : x +nw y ~> x + y := by
-
-  poison_unroll x y => a b
-
-  simp [iN_unwrap_inst]
-  if h1 : (a.saddOverflow b ∨ a.uaddOverflow b) then
-    simp [h1]
-  else
-    simp [h1]
-
-@[grind]
-theorem add_assoc {n} (x y z : iN n)
-    : (x + y) + z = x + (y + z) := by
-
-  poison_unroll x y z => a b c
-  simp [iN_unwrap_inst]
-  rw [BitVec.add_assoc a b c]
-
-@[grind]
-theorem addNsw_not_assoc : ∃ (n : Nat) (x y z : iN n),
-    ¬(x +nsw y) +nsw z <~> x +nsw (y +nsw z) := by
-
-  exists 4
-  exists 6, 5, bitvec (BitVec.neg 7)
-
-  simp [iN_unwrap_inst, BitVec.saddOverflow]
-
-@[grind]
-theorem addNsw_assoc_same_sign {n} {hn : Bits n} (x y z : iN n)
+theorem addNsw_assoc_same_sign {hn : Bits n} (x y z : iN n)
     (h :
       (x ≥ₛ 0) &&& (y ≥ₛ 0) &&& (z ≥ₛ 0) ~> 1 ∨
       (x <ₛ 0) &&& (y <ₛ 0) &&& (z <ₛ 0) ~> 1)
 
-    : (x +nsw y) +nsw z <~> x +nsw (y +nsw z) := by
-
-  poison_unroll x y z => a b c
-  simp [iN_unwrap_inst] at *
-
-  have h' : a.msb = b.msb ∧ b.msb = c.msb := by
-    bv_decide
-
-  rw [BitVec.saddOverflow_chain_assoc_monotone a b c h']
-  rw [BitVec.add_assoc a b c]
-  exact hn
+    : (x +nsw y) +nsw z <~> x +nsw (y +nsw z) := by blast hn
 
 @[grind]
 theorem addNuw_assoc {n} {hn : Bits n} (x y z : iN n)
-    : (x +nuw y) +nuw z <~> x +nuw (y +nuw z) := by
-
-  poison_unroll x y z => a b c
-
-  simp [iN_unwrap_inst]
-  rw [BitVec.uaddOverflow_chain_assoc a b c]
-  rw [BitVec.add_assoc a b c]
-  exact hn
+    : (x +nuw y) +nuw z <~> x +nuw (y +nuw z) := by blast hn
 
 end iN
